src/lang/memory.v
@@ -15,16 +15,14 @@ applies to locations present in both. *)
 Definition valid_slice {A} (V : view) (σ : gmap loc (gmap time A)) :=
   map_Forall (λ ℓ '(MaxNat t, hist), is_Some (hist !! t)) (map_zip V σ).
 
+Definition slice_hist {A} (V : view) (σ : gmap loc (gmap time A)) :
+    gmap loc (option A) :=
+  map_zip_with (λ '(MaxNat t) hist, hist !! t) V σ.
+
 (* For each location in [V] pick the message in the store that it specifies. *)
 Definition slice_of_hist {A} (V : view) (σ : gmap loc (gmap time A)) :
-  gmap loc (gmap time A) :=
-  map_zip_with
-    (λ '(MaxNat t) hist,
-      match hist !! t with
-        Some s => {[ 0 := s ]}
-      | None => ∅ (* The None branch here is never taken. *)
-      end)
-    V σ.
+    gmap loc (gmap time A) :=
+  from_option (λ s, {[ 0 := s ]}) ∅ <$> (slice_hist V σ).
 
 Section slice_of_hist_props.
   Context {A : Type}.
@@ -43,8 +41,8 @@ Section slice_of_hist_props.
     done.
   Qed.
 
-  Lemma slice_of_hist_dom_subset p hists :
-    dom (gset loc) (slice_of_hist p hists) ⊆ dom (gset loc) hists.
+  Lemma slice_hist_dom_subset p hists :
+    dom (gset loc) (slice_hist p hists) ⊆ dom (gset loc) hists.
   Proof.
     rewrite /slice_of_hist.
     intros l.
@@ -55,19 +53,69 @@ Section slice_of_hist_props.
     eexists _. done.
   Qed.
 
+  Lemma slice_hist_lookup_Some CV hists hist ℓ t s :
+    CV !! ℓ = Some (MaxNat t) →
+    hists !! ℓ = Some hist →
+    hist !! t = Some s →
+    slice_hist CV hists !! ℓ = Some (Some s).
+  Proof.
+    intros ?? eq.
+    rewrite /slice_of_hist.
+    apply map_lookup_zip_with_Some.
+    eexists (MaxNat _), _.
+    split_and!; done.
+  Qed.
+
+  Lemma slice_hist_lookup_inv CV hists h ℓ :
+    valid_slice CV hists →
+    slice_hist CV hists !! ℓ = Some h →
+    ∃ t hist m,
+      CV !! ℓ = Some (MaxNat t) ∧
+      hists !! ℓ = Some hist ∧
+      hist !! t = Some m ∧
+      h = Some m.
+  Proof.
+    rewrite /slice_of_hist.
+    intros val ([t] & hist & hl & cvLook & histsLook)%map_lookup_zip_with_Some.
+    eapply map_Forall_lookup_1 in val.
+    2: { apply map_lookup_zip_with_Some. eexists _, _. done. }
+    destruct val as [a histLook].
+    rewrite histLook in hl.
+    naive_solver.
+  Qed.
+
+  Lemma slice_hist_Some V hists ℓ t hist :
+    valid_slice V hists →
+    V !! ℓ = Some (MaxNat t) →
+    hists !! ℓ = Some hist →
+    ∃ (a : A), hist !! t = Some a ∧
+      slice_hist V hists !! ℓ = Some (Some a).
+  Proof.
+    intros val vLook histsLook.
+    eapply valid_slice_lookup in val as [a look]; try done.
+    exists a. split; first done.
+    eapply slice_hist_lookup_Some; done.
+  Qed.
+
+  Lemma slice_of_hist_dom p hists :
+    dom (gset loc) (slice_of_hist p hists) =
+      dom (gset loc) p ∩ dom (gset loc) hists.
+  Proof.
+    rewrite /slice_of_hist dom_fmap_L dom_map_zip_with_L. done.
+  Qed.
+
+  Lemma slice_of_hist_dom_subset p hists :
+    dom (gset loc) (slice_of_hist p hists) ⊆ dom (gset loc) hists.
+  Proof. rewrite /slice_of_hist dom_fmap_L. apply slice_hist_dom_subset. Qed.
+
   Lemma slice_of_hist_lookup_Some CV hists hist ℓ t s :
     CV !! ℓ = Some (MaxNat t) →
     hists !! ℓ = Some hist →
     hist !! t = Some s →
     slice_of_hist CV hists !! ℓ = Some {[0 := s]}.
   Proof.
-    intros ?? eq.
-    rewrite /slice_of_hist.
-    apply map_lookup_zip_with_Some.
-    eexists (MaxNat _), _.
-    split_and!; try done.
-    rewrite eq.
-    done.
+    intros ?? eq. rewrite /slice_of_hist lookup_fmap.
+    erewrite slice_hist_lookup_Some; done.
   Qed.
 
   Lemma slice_of_hist_lookup_inv CV hists h ℓ :
@@ -80,11 +128,8 @@ Section slice_of_hist_props.
       h = {[ 0 := m ]} .
   Proof.
     rewrite /slice_of_hist.
-    intros val ([t] & hist & hl & cvLook & histsLook)%map_lookup_zip_with_Some.
-    eapply map_Forall_lookup_1 in val.
-    2: { apply map_lookup_zip_with_Some. eexists _, _. done. }
-    destruct val as [a histLook].
-    rewrite histLook in hl.
+    intros val (? & ? & slice)%lookup_fmap_Some.
+    pose proof (slice_hist_lookup_inv _ _ _ _ val slice).
     naive_solver.
   Qed.
 
@@ -206,11 +251,12 @@ Section consistent_cut.
   Lemma consistent_cut_lookup_slice CV σ ℓ :
     consistent_cut CV σ → slice_of_store CV σ !! ℓ = None → CV !! ℓ = None.
   Proof.
-    rewrite -!not_elem_of_dom. rewrite /slice_of_store.
+    rewrite -!not_elem_of_dom.
+    rewrite /slice_of_store.
     rewrite dom_fmap.
-    rewrite /slice_of_hist.
-    rewrite dom_map_zip_with.
-    intros ?%consistent_cut_subseteq_dom. set_solver.
+    rewrite slice_of_hist_dom.
+    intros ?%consistent_cut_subseteq_dom.
+    set_solver.
   Qed.
 
   Lemma consistent_cut_extract CV store ℓ t hist msg :
@@ -271,6 +317,7 @@ Section consistent_cut.
       hist = {[0 := discard_msg_views msg']}.
   Proof.
     rewrite /slice_of_store /slice_of_hist map_fmap_zip_with.
+    rewrite map_fmap_zip_with.
     intros ([t'] & h & -> & ? & ?)%map_lookup_zip_with_Some histLook.
     exists t', h.
     destruct (h !! t') as [m|]; last naive_solver.
@@ -288,6 +335,7 @@ Section consistent_cut.
            (msg_val <$> h !! t) = Some (msg_val msg).
   Proof.
     rewrite /slice_of_store /slice_of_hist map_fmap_zip_with.
+    rewrite map_fmap_zip_with.
     intros ([t] & h & eq & ? & ?)%map_lookup_zip_with_Some.
     exists t, h.
     split_and!; [done | done |].
